ironfleet/src/Dafny/Distributed/Services/Lock/LockDistributedSystem.i.dfy
@@ -1,7 +1,8 @@
 include "../../Impl/Lock/Host.i.dfy"
+include "../../Common/Framework/DistributedSystem.s.dfy"
 
 module Lock_DistributedSystem_i refines DistributedSystem_s {
 
-    import opened H_s = Host_i
+    import H_s = Host_i
 
 }
